$$c = \frac{H_1 \cdot \bar{H_2}}{\sqrt{(H_1\cdot \bar{H_1}) (H_2 \cdot \bar{H_2}) }}$$
#### Error propagation
$$\frac{\partial c}{\partial H_1} = \frac{H_1(H_2)}{}$$

$$f = X\cdot Y = x_0y_0 + x_1y_1 + \cdots + x_n y_n$$
$$\sigma_f^2 = y_0^2\sigma_{x_0}^2 + \cdots + y_n^2 \sigma_{x_n}^2 + x_0^2\sigma_{y_0}^2 + \cdots + x_n^2 \sigma_{y_n}^2 = Y°2 \cdot \Sigma_x^2 + X°2 \cdot \Sigma_y^2  $$


### test
$$(a+bi)(c-di) = ac - adi +bci +bd = ac+bd + i(bc-ad)$$

$$V_M = V_R-V_g$$ $$V_C = V_g-V_R = -(-V_g-V_R) = -V_M$$